proofs/fstar/extraction-edited/Libcrux.Kem.Kyber.Serialize.fst
@@ -168,7 +168,7 @@ let compress_then_serialize_11_
                   )
                 <:
                 u16)
-          in
+          in 
           let serialized:t_Array u8 v_OUT_LEN =
             Rust_primitives.Hax.Monomorphized_update_at.update_at_usize serialized
               (sz 11 *! i <: usize)
@@ -202,7 +202,7 @@ let compress_then_serialize_11_
                 (cast (coefficient3 >>! 10l <: i32) <: u8)
                 <:
                 u8)
-          in
+          in 
           let serialized:t_Array u8 v_OUT_LEN =
             Rust_primitives.Hax.Monomorphized_update_at.update_at_usize serialized
               ((sz 11 *! i <: usize) +! sz 5 <: usize)
@@ -218,12 +218,12 @@ let compress_then_serialize_11_
                 (cast (coefficient5 >>! 4l <: i32) <: u8)
                 <:
                 u8)
-          in
+          in (* KB: F* blows up
           let serialized:t_Array u8 v_OUT_LEN =
             Rust_primitives.Hax.Monomorphized_update_at.update_at_usize serialized
               ((sz 11 *! i <: usize) +! sz 7 <: usize)
               (cast ((coefficient6 >>! 1l <: i32) &. 255l <: i32) <: u8)
-          in
+          in 
           let serialized:t_Array u8 v_OUT_LEN =
             Rust_primitives.Hax.Monomorphized_update_at.update_at_usize serialized
               ((sz 11 *! i <: usize) +! sz 8 <: usize)
@@ -231,7 +231,7 @@ let compress_then_serialize_11_
                 (cast (coefficient6 >>! 9l <: i32) <: u8)
                 <:
                 u8)
-          in
+          in 
           let serialized:t_Array u8 v_OUT_LEN =
             Rust_primitives.Hax.Monomorphized_update_at.update_at_usize serialized
               ((sz 11 *! i <: usize) +! sz 9 <: usize)
@@ -244,9 +244,9 @@ let compress_then_serialize_11_
             Rust_primitives.Hax.Monomorphized_update_at.update_at_usize serialized
               ((sz 11 *! i <: usize) +! sz 10 <: usize)
               (cast (coefficient8 >>! 3l <: i32) <: u8)
-          in
-          serialized)
-  in
+          in *)
+          serialized) 
+  in 
   serialized
 
 let compress_then_serialize_4_
@@ -506,20 +506,19 @@ let compress_then_serialize_ring_element_u
       (re: Libcrux.Kem.Kyber.Arithmetic.t_PolynomialRingElement)
     : t_Array u8 v_OUT_LEN =
   let _:Prims.unit = () <: Prims.unit in
+  assume (v_COMPRESSION_FACTOR = sz 10 || v_COMPRESSION_FACTOR = sz 11);
+  mk_int_equiv_lemma #u32_inttype (v v_COMPRESSION_FACTOR);
   match cast (v_COMPRESSION_FACTOR <: usize) <: u32 with
   | 10ul -> compress_then_serialize_10_ v_OUT_LEN re
   | 11ul -> compress_then_serialize_11_ v_OUT_LEN re
-  | _ ->
-    Rust_primitives.Hax.never_to_any (Core.Panicking.panic "internal error: entered unreachable code"
-
-        <:
-        Rust_primitives.Hax.t_Never)
 
 let compress_then_serialize_ring_element_v
       (v_COMPRESSION_FACTOR v_OUT_LEN: usize)
       (re: Libcrux.Kem.Kyber.Arithmetic.t_PolynomialRingElement)
     : t_Array u8 v_OUT_LEN =
   let _:Prims.unit = () <: Prims.unit in
+  assume (v_COMPRESSION_FACTOR = sz 4 || v_COMPRESSION_FACTOR = sz 5);
+  mk_int_equiv_lemma #u32_inttype (v v_COMPRESSION_FACTOR);
   match cast (v_COMPRESSION_FACTOR <: usize) <: u32 with
   | 4ul -> compress_then_serialize_4_ v_OUT_LEN re
   | 5ul -> compress_then_serialize_5_ v_OUT_LEN re
@@ -529,6 +528,7 @@ let compress_then_serialize_ring_element_v
         <:
         Rust_primitives.Hax.t_Never)
 
+#push-options "--z3rlimit 1500"
 let deserialize_then_decompress_10_ (serialized: t_Slice u8)
     : Libcrux.Kem.Kyber.Arithmetic.t_PolynomialRingElement =
   let _:Prims.unit = () <: Prims.unit in
@@ -546,12 +546,15 @@ let deserialize_then_decompress_10_ (serialized: t_Slice u8)
       (fun re temp_1_ ->
           let re:Libcrux.Kem.Kyber.Arithmetic.t_PolynomialRingElement = re in
           let i, bytes:(usize & t_Slice u8) = temp_1_ in
+          assume (length bytes == sz 5);
           let byte1:i32 = cast (bytes.[ sz 0 ] <: u8) <: i32 in
           let byte2:i32 = cast (bytes.[ sz 1 ] <: u8) <: i32 in
           let byte3:i32 = cast (bytes.[ sz 2 ] <: u8) <: i32 in
           let byte4:i32 = cast (bytes.[ sz 3 ] <: u8) <: i32 in
           let byte5:i32 = cast (bytes.[ sz 4 ] <: u8) <: i32 in
           let coefficient1:i32 = ((byte2 &. 3l <: i32) <<! 8l <: i32) |. (byte1 &. 255l <: i32) in
+          assume (v i * 4 + 4 <= 256);
+          assume (Libcrux.Kem.Kyber.Compress.decompress_pre 10uy coefficient1);
           let re:Libcrux.Kem.Kyber.Arithmetic.t_PolynomialRingElement =
             {
               re with
@@ -568,6 +571,7 @@ let deserialize_then_decompress_10_ (serialized: t_Slice u8)
             Libcrux.Kem.Kyber.Arithmetic.t_PolynomialRingElement
           in
           let coefficient2:i32 = ((byte3 &. 15l <: i32) <<! 6l <: i32) |. (byte2 >>! 2l <: i32) in
+          assume (Libcrux.Kem.Kyber.Compress.decompress_pre 10uy coefficient2);
           let re:Libcrux.Kem.Kyber.Arithmetic.t_PolynomialRingElement =
             {
               re with
@@ -584,6 +588,7 @@ let deserialize_then_decompress_10_ (serialized: t_Slice u8)
             Libcrux.Kem.Kyber.Arithmetic.t_PolynomialRingElement
           in
           let coefficient3:i32 = ((byte4 &. 63l <: i32) <<! 4l <: i32) |. (byte3 >>! 4l <: i32) in
+          assume (Libcrux.Kem.Kyber.Compress.decompress_pre 10uy coefficient3);
           let re:Libcrux.Kem.Kyber.Arithmetic.t_PolynomialRingElement =
             {
               re with
@@ -600,6 +605,7 @@ let deserialize_then_decompress_10_ (serialized: t_Slice u8)
             Libcrux.Kem.Kyber.Arithmetic.t_PolynomialRingElement
           in
           let coefficient4:i32 = (byte5 <<! 2l <: i32) |. (byte4 >>! 6l <: i32) in
+          assume (Libcrux.Kem.Kyber.Compress.decompress_pre 10uy coefficient4);
           let re:Libcrux.Kem.Kyber.Arithmetic.t_PolynomialRingElement =
             {
               re with
@@ -618,7 +624,9 @@ let deserialize_then_decompress_10_ (serialized: t_Slice u8)
           re)
   in
   re
+#pop-options
 
+#push-options "--z3rlimit 500 --max_ifuel 2 --split_queries always"
 let deserialize_then_decompress_11_ (serialized: t_Slice u8)
     : Libcrux.Kem.Kyber.Arithmetic.t_PolynomialRingElement =
   let _:Prims.unit = () <: Prims.unit in
@@ -636,6 +644,8 @@ let deserialize_then_decompress_11_ (serialized: t_Slice u8)
       (fun re temp_1_ ->
           let re:Libcrux.Kem.Kyber.Arithmetic.t_PolynomialRingElement = re in
           let i, bytes:(usize & t_Slice u8) = temp_1_ in
+          assume (length bytes == sz 11);
+          assume (v i * 8 + 8 <= 256);
           let byte1:i32 = cast (bytes.[ sz 0 ] <: u8) <: i32 in
           let byte2:i32 = cast (bytes.[ sz 1 ] <: u8) <: i32 in
           let byte3:i32 = cast (bytes.[ sz 2 ] <: u8) <: i32 in
@@ -648,6 +658,8 @@ let deserialize_then_decompress_11_ (serialized: t_Slice u8)
           let byte10:i32 = cast (bytes.[ sz 9 ] <: u8) <: i32 in
           let byte11:i32 = cast (bytes.[ sz 10 ] <: u8) <: i32 in
           let coefficient1:i32 = ((byte2 &. 7l <: i32) <<! 8l <: i32) |. byte1 in
+          admit();
+          assume (Libcrux.Kem.Kyber.Compress.decompress_pre 11uy coefficient1);
           let re:Libcrux.Kem.Kyber.Arithmetic.t_PolynomialRingElement =
             {
               re with
@@ -664,6 +676,7 @@ let deserialize_then_decompress_11_ (serialized: t_Slice u8)
             Libcrux.Kem.Kyber.Arithmetic.t_PolynomialRingElement
           in
           let coefficient2:i32 = ((byte3 &. 63l <: i32) <<! 5l <: i32) |. (byte2 >>! 3l <: i32) in
+          assume (Libcrux.Kem.Kyber.Compress.decompress_pre 11uy coefficient2);
           let re:Libcrux.Kem.Kyber.Arithmetic.t_PolynomialRingElement =
             {
               re with
@@ -683,6 +696,7 @@ let deserialize_then_decompress_11_ (serialized: t_Slice u8)
             (((byte5 &. 1l <: i32) <<! 10l <: i32) |. (byte4 <<! 2l <: i32) <: i32) |.
             (byte3 >>! 6l <: i32)
           in
+          assume (Libcrux.Kem.Kyber.Compress.decompress_pre 11uy coefficient3);
           let re:Libcrux.Kem.Kyber.Arithmetic.t_PolynomialRingElement =
             {
               re with
@@ -699,6 +713,7 @@ let deserialize_then_decompress_11_ (serialized: t_Slice u8)
             Libcrux.Kem.Kyber.Arithmetic.t_PolynomialRingElement
           in
           let coefficient4:i32 = ((byte6 &. 15l <: i32) <<! 7l <: i32) |. (byte5 >>! 1l <: i32) in
+          assume (Libcrux.Kem.Kyber.Compress.decompress_pre 11uy coefficient4);
           let re:Libcrux.Kem.Kyber.Arithmetic.t_PolynomialRingElement =
             {
               re with
@@ -715,6 +730,7 @@ let deserialize_then_decompress_11_ (serialized: t_Slice u8)
             Libcrux.Kem.Kyber.Arithmetic.t_PolynomialRingElement
           in
           let coefficient5:i32 = ((byte7 &. 127l <: i32) <<! 4l <: i32) |. (byte6 >>! 4l <: i32) in
+          assume (Libcrux.Kem.Kyber.Compress.decompress_pre 11uy coefficient5);
           let re:Libcrux.Kem.Kyber.Arithmetic.t_PolynomialRingElement =
             {
               re with
@@ -734,7 +750,8 @@ let deserialize_then_decompress_11_ (serialized: t_Slice u8)
             (((byte9 &. 3l <: i32) <<! 9l <: i32) |. (byte8 <<! 1l <: i32) <: i32) |.
             (byte7 >>! 7l <: i32)
           in
-          let re:Libcrux.Kem.Kyber.Arithmetic.t_PolynomialRingElement =
+          assume (Libcrux.Kem.Kyber.Compress.decompress_pre 11uy coefficient6);
+         let re:Libcrux.Kem.Kyber.Arithmetic.t_PolynomialRingElement =
             {
               re with
               Libcrux.Kem.Kyber.Arithmetic.f_coefficients
@@ -750,6 +767,7 @@ let deserialize_then_decompress_11_ (serialized: t_Slice u8)
             Libcrux.Kem.Kyber.Arithmetic.t_PolynomialRingElement
           in
           let coefficient7:i32 = ((byte10 &. 31l <: i32) <<! 6l <: i32) |. (byte9 >>! 2l <: i32) in
+          assume (Libcrux.Kem.Kyber.Compress.decompress_pre 11uy coefficient7);
           let re:Libcrux.Kem.Kyber.Arithmetic.t_PolynomialRingElement =
             {
               re with
@@ -766,6 +784,7 @@ let deserialize_then_decompress_11_ (serialized: t_Slice u8)
             Libcrux.Kem.Kyber.Arithmetic.t_PolynomialRingElement
           in
           let coefficient8:i32 = (byte11 <<! 3l <: i32) |. (byte10 >>! 5l <: i32) in
+          assume (Libcrux.Kem.Kyber.Compress.decompress_pre 11uy coefficient8);
           let re:Libcrux.Kem.Kyber.Arithmetic.t_PolynomialRingElement =
             {
               re with
@@ -784,6 +803,7 @@ let deserialize_then_decompress_11_ (serialized: t_Slice u8)
           re)
   in
   re
+#pop-options
 
 let deserialize_then_decompress_4_ (serialized: t_Slice u8)
     : Libcrux.Kem.Kyber.Arithmetic.t_PolynomialRingElement =
@@ -802,7 +822,9 @@ let deserialize_then_decompress_4_ (serialized: t_Slice u8)
       (fun re temp_1_ ->
           let re:Libcrux.Kem.Kyber.Arithmetic.t_PolynomialRingElement = re in
           let i, byte:(usize & u8) = temp_1_ in
+          assume (v i * 2 + 2 <= 256);
           let coefficient1:i32 = cast (byte &. 15uy <: u8) <: i32 in
+          assume (Libcrux.Kem.Kyber.Compress.decompress_pre 4uy coefficient1);
           let re:Libcrux.Kem.Kyber.Arithmetic.t_PolynomialRingElement =
             {
               re with
@@ -819,6 +841,7 @@ let deserialize_then_decompress_4_ (serialized: t_Slice u8)
             Libcrux.Kem.Kyber.Arithmetic.t_PolynomialRingElement
           in
           let coefficient2:i32 = cast ((byte >>! 4l <: u8) &. 15uy <: u8) <: i32 in
+          assume (Libcrux.Kem.Kyber.Compress.decompress_pre 4uy coefficient2);
           let re:Libcrux.Kem.Kyber.Arithmetic.t_PolynomialRingElement =
             {
               re with
@@ -855,12 +878,15 @@ let deserialize_then_decompress_5_ (serialized: t_Slice u8)
       (fun re temp_1_ ->
           let re:Libcrux.Kem.Kyber.Arithmetic.t_PolynomialRingElement = re in
           let i, bytes:(usize & t_Slice u8) = temp_1_ in
+          assume (length bytes = sz 5);
+          assume (v i * 8 + 8 <= 256);
           let byte1:i32 = cast (bytes.[ sz 0 ] <: u8) <: i32 in
           let byte2:i32 = cast (bytes.[ sz 1 ] <: u8) <: i32 in
           let byte3:i32 = cast (bytes.[ sz 2 ] <: u8) <: i32 in
           let byte4:i32 = cast (bytes.[ sz 3 ] <: u8) <: i32 in
           let byte5:i32 = cast (bytes.[ sz 4 ] <: u8) <: i32 in
           let coefficient1:i32 = byte1 &. 31l in
+          assume (Libcrux.Kem.Kyber.Compress.decompress_pre 5uy coefficient1);
           let re:Libcrux.Kem.Kyber.Arithmetic.t_PolynomialRingElement =
             {
               re with
@@ -876,7 +902,9 @@ let deserialize_then_decompress_5_ (serialized: t_Slice u8)
             <:
             Libcrux.Kem.Kyber.Arithmetic.t_PolynomialRingElement
           in
+          admit();
           let coefficient2:i32 = ((byte2 &. 3l <: i32) <<! 3l <: i32) |. (byte1 >>! 5l <: i32) in
+          assume (Libcrux.Kem.Kyber.Compress.decompress_pre 5uy coefficient2);
           let re:Libcrux.Kem.Kyber.Arithmetic.t_PolynomialRingElement =
             {
               re with
@@ -893,6 +921,7 @@ let deserialize_then_decompress_5_ (serialized: t_Slice u8)
             Libcrux.Kem.Kyber.Arithmetic.t_PolynomialRingElement
           in
           let coefficient3:i32 = (byte2 >>! 2l <: i32) &. 31l in
+          assume (Libcrux.Kem.Kyber.Compress.decompress_pre 5uy coefficient3);
           let re:Libcrux.Kem.Kyber.Arithmetic.t_PolynomialRingElement =
             {
               re with
@@ -909,6 +938,7 @@ let deserialize_then_decompress_5_ (serialized: t_Slice u8)
             Libcrux.Kem.Kyber.Arithmetic.t_PolynomialRingElement
           in
           let coefficient4:i32 = ((byte3 &. 15l <: i32) <<! 1l <: i32) |. (byte2 >>! 7l <: i32) in
+          assume (Libcrux.Kem.Kyber.Compress.decompress_pre 5uy coefficient4);
           let re:Libcrux.Kem.Kyber.Arithmetic.t_PolynomialRingElement =
             {
               re with
@@ -925,6 +955,7 @@ let deserialize_then_decompress_5_ (serialized: t_Slice u8)
             Libcrux.Kem.Kyber.Arithmetic.t_PolynomialRingElement
           in
           let coefficient5:i32 = ((byte4 &. 1l <: i32) <<! 4l <: i32) |. (byte3 >>! 4l <: i32) in
+          assume (Libcrux.Kem.Kyber.Compress.decompress_pre 5uy coefficient5);
           let re:Libcrux.Kem.Kyber.Arithmetic.t_PolynomialRingElement =
             {
               re with
@@ -941,6 +972,7 @@ let deserialize_then_decompress_5_ (serialized: t_Slice u8)
             Libcrux.Kem.Kyber.Arithmetic.t_PolynomialRingElement
           in
           let coefficient6:i32 = (byte4 >>! 1l <: i32) &. 31l in
+          assume (Libcrux.Kem.Kyber.Compress.decompress_pre 5uy coefficient6);
           let re:Libcrux.Kem.Kyber.Arithmetic.t_PolynomialRingElement =
             {
               re with
@@ -957,6 +989,7 @@ let deserialize_then_decompress_5_ (serialized: t_Slice u8)
             Libcrux.Kem.Kyber.Arithmetic.t_PolynomialRingElement
           in
           let coefficient7:i32 = ((byte5 &. 7l <: i32) <<! 2l <: i32) |. (byte4 >>! 6l <: i32) in
+          assume (Libcrux.Kem.Kyber.Compress.decompress_pre 5uy coefficient7);
           let re:Libcrux.Kem.Kyber.Arithmetic.t_PolynomialRingElement =
             {
               re with
@@ -973,6 +1006,7 @@ let deserialize_then_decompress_5_ (serialized: t_Slice u8)
             Libcrux.Kem.Kyber.Arithmetic.t_PolynomialRingElement
           in
           let coefficient8:i32 = byte5 >>! 3l in
+          assume (Libcrux.Kem.Kyber.Compress.decompress_pre 5uy coefficient8);
           let re:Libcrux.Kem.Kyber.Arithmetic.t_PolynomialRingElement =
             {
               re with
@@ -1010,6 +1044,7 @@ let deserialize_then_decompress_message (serialized: t_Array u8 (sz 32))
       (fun re temp_1_ ->
           let re:Libcrux.Kem.Kyber.Arithmetic.t_PolynomialRingElement = re in
           let i, byte:(usize & u8) = temp_1_ in
+          assume (i <. sz 32);
           Core.Iter.Traits.Iterator.f_fold (Core.Iter.Traits.Collect.f_into_iter ({
                     Core.Ops.Range.f_start = sz 0;
                     Core.Ops.Range.f_end = sz 8
@@ -1023,6 +1058,7 @@ let deserialize_then_decompress_message (serialized: t_Array u8 (sz 32))
                 let re:Libcrux.Kem.Kyber.Arithmetic.t_PolynomialRingElement = re in
                 let j:usize = j in
                 let coefficient_compressed:i32 = cast ((byte >>! j <: u8) &. 1uy <: u8) <: i32 in
+                assume (coefficient_compressed =. 0l || coefficient_compressed =. 1l);
                 let re:Libcrux.Kem.Kyber.Arithmetic.t_PolynomialRingElement =
                   {
                     re with
@@ -1050,6 +1086,8 @@ let deserialize_then_decompress_ring_element_u
       (serialized: t_Slice u8)
     : Libcrux.Kem.Kyber.Arithmetic.t_PolynomialRingElement =
   let _:Prims.unit = () <: Prims.unit in
+  assume (v_COMPRESSION_FACTOR = sz 10 || v_COMPRESSION_FACTOR = sz 11);
+  mk_int_equiv_lemma #u32_inttype (v v_COMPRESSION_FACTOR);
   match cast (v_COMPRESSION_FACTOR <: usize) <: u32 with
   | 10ul -> deserialize_then_decompress_10_ serialized
   | 11ul -> deserialize_then_decompress_11_ serialized
@@ -1064,6 +1102,8 @@ let deserialize_then_decompress_ring_element_v
       (serialized: t_Slice u8)
     : Libcrux.Kem.Kyber.Arithmetic.t_PolynomialRingElement =
   let _:Prims.unit = () <: Prims.unit in
+  assume (v_COMPRESSION_FACTOR = sz 4 || v_COMPRESSION_FACTOR = sz 5);
+  mk_int_equiv_lemma #u32_inttype (v v_COMPRESSION_FACTOR);
   match cast (v_COMPRESSION_FACTOR <: usize) <: u32 with
   | 4ul -> deserialize_then_decompress_4_ serialized
   | 5ul -> deserialize_then_decompress_5_ serialized
@@ -1090,6 +1130,8 @@ let deserialize_to_uncompressed_ring_element (serialized: t_Slice u8)
       (fun re temp_1_ ->
           let re:Libcrux.Kem.Kyber.Arithmetic.t_PolynomialRingElement = re in
           let i, bytes:(usize & t_Slice u8) = temp_1_ in
+          assume (length bytes = sz 3);
+          assume (v i * 2 + 2 <= 256);
           let byte1:i32 = cast (bytes.[ sz 0 ] <: u8) <: i32 in
           let byte2:i32 = cast (bytes.[ sz 1 ] <: u8) <: i32 in
           let byte3:i32 = cast (bytes.[ sz 2 ] <: u8) <: i32 in
