proofs/fstar/extraction/Libcrux.Kem.Kyber.Compress.fst
@@ -10,17 +10,14 @@ let compress_message_coefficient (fe: u16)
         fun result ->
           let result:u8 = result in
           Hax_lib.implies ((833us <=. fe <: bool) && (fe <=. 2596us <: bool))
-            (fun _ -> result =. 1uy <: bool) &&
+            (result =. 1uy <: bool) &&
           Hax_lib.implies (~.((833us <=. fe <: bool) && (fe <=. 2596us <: bool)) <: bool)
-            (fun _ -> result =. 0uy <: bool)) =
+            (result =. 0uy <: bool)) =
   let (shifted: i16):i16 = 1664s -! (cast (fe <: u16) <: i16) in
   let mask:i16 = shifted >>! 15l in
   let shifted_to_positive:i16 = mask ^. shifted in
-  assume (shifted_to_positive >=. 0s);
   let shifted_positive_in_range:i16 = shifted_to_positive -! 832s in
-  let res = cast ((shifted_positive_in_range >>! 15l <: i16) &. 1s <: i16) <: u8 in
-  admit();
-  res
+  cast ((shifted_positive_in_range >>! 15l <: i16) &. 1s <: i16) <: u8
 
 let compress_ciphertext_coefficient (coefficient_bits: u8) (fe: u16)
     : Prims.Pure i32
@@ -47,15 +44,13 @@ let compress_ciphertext_coefficient (coefficient_bits: u8) (fe: u16)
   <:
   i32
 
-let decompress_pre (coefficient_bits: u8) (fe: i32) = 
+let decompress_ciphertext_coefficient (coefficient_bits: u8) (fe: i32)
+    : Prims.Pure i32
+      (requires
         (coefficient_bits =. 4uy || coefficient_bits =. 5uy || coefficient_bits =. 10uy ||
         coefficient_bits =. 11uy) &&
         fe >=. 0l &&
-        fe <. (Core.Num.impl__i32__pow 2l (cast (coefficient_bits <: u8) <: u32) <: i32)
-
-let decompress_ciphertext_coefficient (coefficient_bits: u8) (fe: i32)
-    : Prims.Pure i32
-      (requires (decompress_pre coefficient_bits fe))
+        fe <. (Core.Num.impl__i32__pow 2l (cast (coefficient_bits <: u8) <: u32) <: i32))
       (ensures
         fun result ->
           let result:i32 = result in
@@ -65,11 +60,9 @@ let decompress_ciphertext_coefficient (coefficient_bits: u8) (fe: i32)
   let decompressed:u32 =
     (cast (fe <: i32) <: u32) *! (cast (Libcrux.Kem.Kyber.Constants.v_FIELD_MODULUS <: i32) <: u32)
   in
-  admit();
   let decompressed:u32 = (decompressed <<! 1l <: u32) +! (1ul <<! coefficient_bits <: u32) in
   let decompressed:u32 = decompressed >>! (coefficient_bits +! 1uy <: u8) in
-  let res = cast (decompressed <: u32) <: i32 in
-  res
+  cast (decompressed <: u32) <: i32
 
 let decompress_message_coefficient (fe: i32)
     : Prims.Pure i32 (requires fe =. 0l || fe =. 1l) (fun _ -> Prims.l_True) =
