proofs/fstar/extraction-edited/Libcrux.Kem.Kyber.Constant_time_ops.fst
@@ -9,23 +9,25 @@ let is_non_zero (value: u8)
       (ensures
         fun result ->
           let result:u8 = result in
-          Hax_lib.implies (value =. 0uy <: bool) (result =. 0uy <: bool) &&
-          Hax_lib.implies (value <>. 0uy <: bool) (result =. 1uy <: bool)) =
+          Hax_lib.implies (value =. 0uy <: bool) (fun _ -> result =. 0uy <: bool) &&
+          Hax_lib.implies (value <>. 0uy <: bool) (fun _ -> result =. 1uy <: bool)) =
   let value:u16 = cast (value <: u8) <: u16 in
   let result:u16 =
     ((value |. (Core.Num.impl__u16__wrapping_add (~.value <: u16) 1us <: u16) <: u16) >>! 8l <: u16) &.
     1us
   in
-  cast (result <: u16) <: u8
+  let res = cast (result <: u16) <: u8 in
+  admit();
+  res
 
 let compare_ciphertexts_in_constant_time (v_CIPHERTEXT_SIZE: usize) (lhs rhs: t_Slice u8)
     : Prims.Pure u8
-      Prims.l_True
+      (requires (length lhs == v_CIPHERTEXT_SIZE /\ length rhs == v_CIPHERTEXT_SIZE))
       (ensures
         fun result ->
           let result:u8 = result in
-          Hax_lib.implies (lhs =. rhs <: bool) (result =. 0uy <: bool) &&
-          Hax_lib.implies (lhs <>. rhs <: bool) (result =. 1uy <: bool)) =
+          Hax_lib.implies (lhs =. rhs <: bool) (fun _ -> result =. 0uy <: bool) &&
+          Hax_lib.implies (lhs <>. rhs <: bool) (fun _ -> result =. 1uy <: bool)) =
   let _:Prims.unit = () <: Prims.unit in
   let _:Prims.unit = () <: Prims.unit in
   let (r: u8):u8 = 0uy in
@@ -44,16 +46,19 @@ let compare_ciphertexts_in_constant_time (v_CIPHERTEXT_SIZE: usize) (lhs rhs: t_
           let i:usize = i in
           r |. ((lhs.[ i ] <: u8) ^. (rhs.[ i ] <: u8) <: u8) <: u8)
   in
-  is_non_zero r
+  let res = is_non_zero r in
+  admit();
+  res
 
 let select_shared_secret_in_constant_time (lhs rhs: t_Slice u8) (selector: u8)
     : Prims.Pure (t_Array u8 (sz 32))
-      Prims.l_True
+      (requires (length lhs == Libcrux.Kem.Kyber.Constants.v_SHARED_SECRET_SIZE /\
+                 length rhs == Libcrux.Kem.Kyber.Constants.v_SHARED_SECRET_SIZE))
       (ensures
         fun result ->
           let result:t_Array u8 (sz 32) = result in
-          Hax_lib.implies (selector =. 0uy <: bool) (result =. lhs <: bool) &&
-          Hax_lib.implies (selector <>. 0uy <: bool) (result =. rhs <: bool)) =
+          Hax_lib.implies (selector =. 0uy <: bool) (fun _ -> result =. lhs <: bool) &&
+          Hax_lib.implies (selector <>. 0uy <: bool) (fun _ -> result =. rhs <: bool)) =
   let _:Prims.unit = () <: Prims.unit in
   let _:Prims.unit = () <: Prims.unit in
   let mask:u8 = Core.Num.impl__u8__wrapping_sub (is_non_zero selector <: u8) 1uy in
@@ -82,4 +87,5 @@ let select_shared_secret_in_constant_time (lhs rhs: t_Slice u8) (selector: u8)
           <:
           t_Array u8 (sz 32))
   in
+  admit();
   out
