proofs/fstar/extraction/Libcrux.Kem.Kyber.Kyber768.fst
@@ -78,7 +78,6 @@ let decapsulate_768_
   Libcrux.Kem.Kyber.decapsulate (sz 3) (sz 2400) (sz 1152) (sz 1184) (sz 1088) (sz 1152) (sz 960)
     (sz 128) (sz 10) (sz 4) (sz 320) (sz 2) (sz 128) (sz 2) (sz 128) (sz 1120) secret_key ciphertext
 
-
 let encapsulate_768_
       (public_key: Libcrux.Kem.Kyber.Types.t_KyberPublicKey (sz 1184))
       (randomness: t_Array u8 (sz 32))
@@ -99,4 +98,3 @@ let generate_key_pair_768_ (randomness: t_Array u8 (sz 64))
     (sz 2)
     (sz 128)
     randomness
-
