proofs/fstar/extraction/Libcrux.Kem.Kyber.Ntt.fst
@@ -23,7 +23,6 @@ let v_ZETAS_TIMES_MONTGOMERY_R: t_Array i32 (sz 128) =
   Rust_primitives.Hax.array_of_list list
 
 let ntt_multiply_binomials (a0, a1: (i32 & i32)) (b0, b1: (i32 & i32)) (zeta: i32) : (i32 & i32) =
-  admit(); // Needs preconditions on ranges of all inputs
   Libcrux.Kem.Kyber.Arithmetic.montgomery_reduce ((a0 *! b0 <: i32) +!
       ((Libcrux.Kem.Kyber.Arithmetic.montgomery_reduce (a1 *! b1 <: i32) <: i32) *! zeta <: i32)
       <:
@@ -32,11 +31,11 @@ let ntt_multiply_binomials (a0, a1: (i32 & i32)) (b0, b1: (i32 & i32)) (zeta: i3
   <:
   (i32 & i32)
 
-let invert_ntt_montgomery (v_K: usize) (re: Libcrux.Kem.Kyber.Arithmetic.t_PolynomialRingElement) =
+let invert_ntt_montgomery (v_K: usize) (re: Libcrux.Kem.Kyber.Arithmetic.t_PolynomialRingElement)
+    : Libcrux.Kem.Kyber.Arithmetic.t_PolynomialRingElement =
   let _:Prims.unit = () <: Prims.unit in
   let zeta_i:usize = Libcrux.Kem.Kyber.Constants.v_COEFFICIENTS_IN_RING_ELEMENT /! sz 2 in
   let step:usize = sz 1 <<! 1l in
-  admit(); // Needs many preconditions and is too big, break it up.
   let re, zeta_i:(Libcrux.Kem.Kyber.Arithmetic.t_PolynomialRingElement & usize) =
     Core.Iter.Traits.Iterator.f_fold (Core.Iter.Traits.Collect.f_into_iter ({
               Core.Ops.Range.f_start = sz 0;
@@ -49,7 +48,6 @@ let invert_ntt_montgomery (v_K: usize) (re: Libcrux.Kem.Kyber.Arithmetic.t_Polyn
       (re, zeta_i <: (Libcrux.Kem.Kyber.Arithmetic.t_PolynomialRingElement & usize))
       (fun temp_0_ round ->
           let re, zeta_i:(Libcrux.Kem.Kyber.Arithmetic.t_PolynomialRingElement & usize) = temp_0_ in
-          assume (zeta_i >. sz 1);
           let round:usize = round in
           let zeta_i:usize = zeta_i -! sz 1 in
           let offset:usize = (round *! step <: usize) *! sz 2 in
@@ -584,7 +582,55 @@ let invert_ntt_montgomery (v_K: usize) (re: Libcrux.Kem.Kyber.Arithmetic.t_Polyn
   in
   re
 
-let ntt_binomially_sampled_ring_element (re: Libcrux.Kem.Kyber.Arithmetic.t_PolynomialRingElement) =
+let ntt_binomially_sampled_ring_element (re: Libcrux.Kem.Kyber.Arithmetic.t_PolynomialRingElement)
+    : Prims.Pure Libcrux.Kem.Kyber.Arithmetic.t_PolynomialRingElement
+      (requires
+        Hax_lib.v_forall (fun i ->
+              let i:usize = i in
+              Hax_lib.implies (i <.
+                  (Core.Slice.impl__len (Rust_primitives.unsize re
+                            .Libcrux.Kem.Kyber.Arithmetic.f_coefficients
+                        <:
+                        t_Slice i32)
+                    <:
+                    usize)
+                  <:
+                  bool)
+                ((Core.Num.impl__i32__abs (re.Libcrux.Kem.Kyber.Arithmetic.f_coefficients.[ i ]
+                        <:
+                        i32)
+                    <:
+                    i32) <=.
+                  3l
+                  <:
+                  bool)
+              <:
+              bool))
+      (ensures
+        fun result ->
+          let result:Libcrux.Kem.Kyber.Arithmetic.t_PolynomialRingElement = result in
+          Hax_lib.v_forall (fun i ->
+                let i:usize = i in
+                Hax_lib.implies (i <.
+                    (Core.Slice.impl__len (Rust_primitives.unsize result
+                              .Libcrux.Kem.Kyber.Arithmetic.f_coefficients
+                          <:
+                          t_Slice i32)
+                      <:
+                      usize)
+                    <:
+                    bool)
+                  ((Core.Num.impl__i32__abs (result.Libcrux.Kem.Kyber.Arithmetic.f_coefficients.[ i
+                          ]
+                          <:
+                          i32)
+                      <:
+                      i32) <.
+                    Libcrux.Kem.Kyber.Constants.v_FIELD_MODULUS
+                    <:
+                    bool)
+                <:
+                bool)) =
   let _:Prims.unit = () <: Prims.unit in
   let zeta_i:usize = sz 0 in
   let zeta_i:usize = zeta_i +! sz 1 in
@@ -601,12 +647,10 @@ let ntt_binomially_sampled_ring_element (re: Libcrux.Kem.Kyber.Arithmetic.t_Poly
       (fun re j ->
           let re:Libcrux.Kem.Kyber.Arithmetic.t_PolynomialRingElement = re in
           let j:usize = j in
-          assume (range (v #i32_inttype re.f_coefficients.[j +! sz 128] * (-1600)) i32_inttype);
           let t:i32 =
             (re.Libcrux.Kem.Kyber.Arithmetic.f_coefficients.[ j +! sz 128 <: usize ] <: i32) *!
             (-1600l)
           in
-          assume (range (v #i32_inttype re.f_coefficients.[j] - v t) i32_inttype);
           let re:Libcrux.Kem.Kyber.Arithmetic.t_PolynomialRingElement =
             {
               re with
@@ -620,7 +664,6 @@ let ntt_binomially_sampled_ring_element (re: Libcrux.Kem.Kyber.Arithmetic.t_Poly
             <:
             Libcrux.Kem.Kyber.Arithmetic.t_PolynomialRingElement
           in
-          assume (range (v #i32_inttype re.f_coefficients.[j] + v t) i32_inttype);
           let re:Libcrux.Kem.Kyber.Arithmetic.t_PolynomialRingElement =
             {
               re with
@@ -638,7 +681,6 @@ let ntt_binomially_sampled_ring_element (re: Libcrux.Kem.Kyber.Arithmetic.t_Poly
   in
   let _:Prims.unit = () <: Prims.unit in
   let step:usize = sz 1 <<! 6l in
-  admit(); // Too big, break up.
   let re, zeta_i:(Libcrux.Kem.Kyber.Arithmetic.t_PolynomialRingElement & usize) =
     Core.Iter.Traits.Iterator.f_fold (Core.Iter.Traits.Collect.f_into_iter ({
               Core.Ops.Range.f_start = sz 0;
@@ -651,7 +693,6 @@ let ntt_binomially_sampled_ring_element (re: Libcrux.Kem.Kyber.Arithmetic.t_Poly
       (re, zeta_i <: (Libcrux.Kem.Kyber.Arithmetic.t_PolynomialRingElement & usize))
       (fun temp_0_ round ->
           let re, zeta_i:(Libcrux.Kem.Kyber.Arithmetic.t_PolynomialRingElement & usize) = temp_0_ in
-          assume (v zeta_i < maxint usize_inttype);
           let round:usize = round in
           let zeta_i:usize = zeta_i +! sz 1 in
           let offset:usize = (round *! step <: usize) *! sz 2 in
@@ -1075,7 +1116,51 @@ let ntt_binomially_sampled_ring_element (re: Libcrux.Kem.Kyber.Arithmetic.t_Poly
   in
   re
 
-let ntt_multiply (lhs rhs: Libcrux.Kem.Kyber.Arithmetic.t_PolynomialRingElement) =
+let ntt_multiply (lhs rhs: Libcrux.Kem.Kyber.Arithmetic.t_PolynomialRingElement)
+    : Prims.Pure Libcrux.Kem.Kyber.Arithmetic.t_PolynomialRingElement
+      (requires
+        Hax_lib.v_forall (fun i ->
+              let i:usize = i in
+              Hax_lib.implies (i <. Libcrux.Kem.Kyber.Constants.v_COEFFICIENTS_IN_RING_ELEMENT
+                  <:
+                  bool)
+                (((lhs.Libcrux.Kem.Kyber.Arithmetic.f_coefficients.[ i ] <: i32) >=. 0l <: bool) &&
+                  ((lhs.Libcrux.Kem.Kyber.Arithmetic.f_coefficients.[ i ] <: i32) <. 4096l <: bool) &&
+                  ((Core.Num.impl__i32__abs (rhs.Libcrux.Kem.Kyber.Arithmetic.f_coefficients.[ i ]
+                          <:
+                          i32)
+                      <:
+                      i32) <=.
+                    Libcrux.Kem.Kyber.Constants.v_FIELD_MODULUS
+                    <:
+                    bool))
+              <:
+              bool))
+      (ensures
+        fun result ->
+          let result:Libcrux.Kem.Kyber.Arithmetic.t_PolynomialRingElement = result in
+          Hax_lib.v_forall (fun i ->
+                let i:usize = i in
+                Hax_lib.implies (i <.
+                    (Core.Slice.impl__len (Rust_primitives.unsize result
+                              .Libcrux.Kem.Kyber.Arithmetic.f_coefficients
+                          <:
+                          t_Slice i32)
+                      <:
+                      usize)
+                    <:
+                    bool)
+                  ((Core.Num.impl__i32__abs (result.Libcrux.Kem.Kyber.Arithmetic.f_coefficients.[ i
+                          ]
+                          <:
+                          i32)
+                      <:
+                      i32) <=.
+                    Libcrux.Kem.Kyber.Constants.v_FIELD_MODULUS
+                    <:
+                    bool)
+                <:
+                bool)) =
   let _:Prims.unit = () <: Prims.unit in
   let out:Libcrux.Kem.Kyber.Arithmetic.t_PolynomialRingElement =
     Libcrux.Kem.Kyber.Arithmetic.impl__PolynomialRingElement__ZERO
@@ -1095,7 +1180,6 @@ let ntt_multiply (lhs rhs: Libcrux.Kem.Kyber.Arithmetic.t_PolynomialRingElement)
       (fun out i ->
           let out:Libcrux.Kem.Kyber.Arithmetic.t_PolynomialRingElement = out in
           let i:usize = i in
-          assume (v i * 4 + 4 <= 256);
           let product:(i32 & i32) =
             ntt_multiply_binomials ((lhs.Libcrux.Kem.Kyber.Arithmetic.f_coefficients.[ sz 4 *! i
                     <:
@@ -1223,7 +1307,7 @@ let ntt_vector_u
                     usize)
                   <:
                   bool)
-                (fun _ -> (Core.Num.impl__i32__abs (re.Libcrux.Kem.Kyber.Arithmetic.f_coefficients.[ i ]
+                ((Core.Num.impl__i32__abs (re.Libcrux.Kem.Kyber.Arithmetic.f_coefficients.[ i ]
                         <:
                         i32)
                     <:
@@ -1247,7 +1331,7 @@ let ntt_vector_u
                       usize)
                     <:
                     bool)
-                  (fun _ -> (Core.Num.impl__i32__abs (result.Libcrux.Kem.Kyber.Arithmetic.f_coefficients.[ i
+                  ((Core.Num.impl__i32__abs (result.Libcrux.Kem.Kyber.Arithmetic.f_coefficients.[ i
                           ]
                           <:
                           i32)
